src/Final.v
@@ -1,4 +1,6 @@
-Add LoadPath "../from_compcert".
+Add LoadPath "~/formal/s2sLoop/from_compcert".
+Add LoadPath "~/formal/PilkiLib".
+Add LoadPath "~/formal/s2sLoop/src".
 Require Import Libs.
 Require Import Errors.
 Require Import Polyhedra.
